verification/tests/DepositTests.dfy
@@ -30,14 +30,15 @@ module DepositTests {
   {
     var cfg := Cfg.DummyConfig().(mechanic := FixedPrice(1, 1));
 
-    var (newAmount, newWeight, newTotalDeposited, newTotalSold, newRefund, newAssetsExcess) :=
-      DepositFixedPriceSpec(cfg, 100, 5000, 5000, 150, 1, 1);
+    var amount := 100;
+    var assets := CalculateAssetsSpec(cfg.CalculateWeightedAmountSpec(amount, 150), 1, 1);
+    var (newAmount, newWeight, newTotalDeposited, newTotalSold, newRefund) :=
+      DepositFixedPriceSpec(cfg, amount, 5000, 5000, 150, 1, 1);
 
     assert newRefund == 0;
-    assert newAssetsExcess == 0;
-    assert newAmount == 100;
-    assert newWeight == 100;
-    assert newTotalDeposited == 5000 + 100;
-    assert newTotalSold == 5000 + 100;
+    assert newAmount == amount;
+    assert newWeight == assets == 100;
+    assert newTotalDeposited == 5000 + newAmount;
+    assert newTotalSold == 5000 + newWeight;
   }
 }
