verification/tests/LaunchpadDepositTests.dfy
@@ -4,6 +4,7 @@ module LaunchpadDepositTests {
   import opened Investments
   import opened Discounts
   import opened Launchpad
+  import opened AssetCalculations
   import opened LaunchpadUtils
 
   function DepositWuthoutFixedPriceWithoutRefundTest(): bool {
@@ -26,6 +27,7 @@ module LaunchpadDepositTests {
     assert lp2.totalDeposited == 100000;
     assert lp2.totalSoldTokens == 100000;
     assert lp2.investments[alice] == InvestmentAmount(100000, 100000, 0);
+    assert lp1.IsOngoing(NOW);
 
     var (lp3, amount3, weight3, refund3) := lp2.DepositSpec(alice, 100000, alice, NOW);
     assert amount3 == 100000;
@@ -34,6 +36,7 @@ module LaunchpadDepositTests {
     assert lp3.totalDeposited == 200000;
     assert lp3.totalSoldTokens == 200000;
     assert lp3.investments[alice] == InvestmentAmount(200000, 200000, 0);
+    assert lp3.IsSuccess(cfg.endDate);
     true
   }
 
@@ -57,6 +60,7 @@ module LaunchpadDepositTests {
     assert lp2.totalDeposited == cfg.totalSaleAmount;
     assert lp2.totalSoldTokens == cfg.totalSaleAmount;
     assert lp2.investments[alice] == InvestmentAmount(cfg.totalSaleAmount, cfg.totalSaleAmount, 0);
+    assert lp2.IsSuccess(cfg.endDate);
     true
   }
 
@@ -81,6 +85,7 @@ module LaunchpadDepositTests {
     assert lp2.totalDeposited == cfg.totalSaleAmount / 2;
     assert lp2.totalSoldTokens == cfg.totalSaleAmount;
     assert lp2.investments[alice] == InvestmentAmount(cfg.totalSaleAmount / 2, cfg.totalSaleAmount, 0);
+    assert lp2.IsFailed(cfg.endDate);
     true
   }
 
@@ -98,13 +103,38 @@ module LaunchpadDepositTests {
     assert lp1.IsOngoing(NOW);
 
     var alice := "alice.testnet";
-    var (lp2, amount2, weight2, refund2) := lp1.DepositSpec(alice, cfg.totalSaleAmount + 10000, alice, NOW);
+    var amount := cfg.totalSaleAmount + 10000;
+    var assets := CalculateAssetsSpec(cfg.CalculateWeightedAmountSpec(amount, NOW), 2, 1);
+    var (lp2, amount2, weight2, refund2) := lp1.DepositSpec(alice, amount, alice, NOW);
     assert amount2 == cfg.totalSaleAmount + 10000;
-    // assert weight2 == cfg.totalSaleAmount;
+    assert weight2 == assets;
     assert refund2 == 0;
     assert lp2.totalDeposited == cfg.totalSaleAmount + 10000;
-    // assert lp2.totalSoldTokens == cfg.totalSaleAmount;
-    // assert lp2.investments[alice] == InvestmentAmount(cfg.totalSaleAmount / 2, cfg.totalSaleAmount, 0);
+    assert lp2.totalSoldTokens == assets;
+    assert lp2.investments[alice] == InvestmentAmount(cfg.totalSaleAmount  + 10000, assets, 0);
+
+    var amount_2 := 10000;
+    var assets2 := CalculateAssetsSpec(cfg.CalculateWeightedAmountSpec(amount_2, NOW), 2, 1);
+    var (lp3, amount3, weight3, refund3) := lp2.DepositSpec(alice, amount_2, alice, NOW);
+    assert amount3 == 10000;
+    assert weight3 == assets2;
+    assert refund3 == 0;
+    assert lp3.totalDeposited == cfg.totalSaleAmount + 20000;
+    assert lp3.totalSoldTokens == assets + assets2;
+    assert lp3.investments[alice] == InvestmentAmount(cfg.totalSaleAmount  + 20000, assets + assets2, 0);    
+
+    var bob := "bob.testnet";
+    var amount_3 := 190000;
+    var assets3 := CalculateAssetsSpec(cfg.CalculateWeightedAmountSpec(180000, NOW), 2, 1);
+    var (lp4, amount4, weight4, refund4) := lp3.DepositSpec(bob, amount_3, bob, NOW);
+    assert amount4 == 180000;
+    assert weight4 == assets3 == 90000;
+    assert refund4 == 10000;
+    assert lp4.totalDeposited == 400000;
+    assert lp4.totalSoldTokens == assets + assets2 + assets3 == 200000 == cfg.totalSaleAmount;
+    assert lp4.investments[alice] == InvestmentAmount(cfg.totalSaleAmount  + 20000, assets + assets2, 0);    
+    assert lp4.investments[bob] == InvestmentAmount(180000, assets3, 0);    
+    assert lp4.IsSuccess(cfg.endDate);
     true
   }
 }
